ViperBoogieBasicRel.thy
@@ -1,0 +1,101 @@
+theory ViperBoogieBasicRel
+imports TotalExpressions Boogie_Lang.Semantics ViperBoogieInstantiation
+begin
+
+type_synonym viper_expr = ViperLang.pure_exp
+type_synonym boogie_expr = Lang.expr
+
+fun unop_rel :: "ViperLang.unop \<Rightarrow> Lang.unop"
+  where 
+    "unop_rel ViperLang.Minus = Lang.UMinus"
+  | "unop_rel ViperLang.Not = Lang.Not"
+
+fun binop_rel :: "ViperLang.binop \<Rightarrow> Lang.binop"
+  where 
+    "binop_rel ViperLang.Add = Lang.Add"
+  | "binop_rel ViperLang.Sub = Lang.Sub"
+  | "binop_rel ViperLang.Mult = Lang.Mul"
+  | "binop_rel ViperLang.IntDiv = Lang.Div"
+  | "binop_rel ViperLang.Mod = Lang.Mod"
+  | "binop_rel ViperLang.Eq = Lang.Eq"
+  | "binop_rel ViperLang.Neq = Lang.Neq"
+  | "binop_rel ViperLang.Gt = Lang.Gt"
+  | "binop_rel ViperLang.Gte = Lang.Ge"
+  | "binop_rel ViperLang.Lt = Lang.Lt"
+  | "binop_rel ViperLang.Lte = Lang.Le"
+  | "binop_rel ViperLang.Or = Lang.Or"
+  | "binop_rel ViperLang.BImp = Lang.Imp"
+  | "binop_rel ViperLang.And = Lang.And"
+(* TODO: PermDiv case *)
+
+
+record tr_vpr_bpl =
+  heap_var :: Lang.vname
+  mask_var :: Lang.vname
+(*  mask_read :: "expr \<Rightarrow> expr \<Rightarrow> expr"
+  mask_store :: "expr \<Rightarrow> expr \<Rightarrow> expr \<Rightarrow> expr" *)
+(*  fun_translation :: "string \<Rightarrow> string" *)
+  var_translation :: "ViperLang.var \<rightharpoonup> vname" \<comment>\<open>local Boogie variables\<close>
+  lit_translation :: "ViperLang.lit \<Rightarrow> expr"
+ (*TODO: bound vars*)
+(*  result_var :: "string" *)
+  
+type_synonym 'a vpr_val = "'a ValueAndBasicState.val"
+
+inductive val_rel_vpr_bpl :: "'a vpr_val \<Rightarrow> 'a vbpl_val \<Rightarrow> bool"
+  where
+    IntRel: "val_rel_vpr_bpl (VInt i) (IntV i)"
+  | BoolRel: "val_rel_vpr_bpl (VBool b) (BoolV b)"
+  | RefRel: "val_rel_vpr_bpl (VRef r) (AbsV (ARef r))"
+  | DomainRel: "val_rel_vpr_bpl (VAbs a) (AbsV (ADomainVal a))"
+  | PermRel: "val_rel_vpr_bpl (VPerm r) (RealV (real_of_rat r))"
+                                             
+type_synonym 'a bpl_heap_ty = "ref \<Rightarrow> 'a vb_field \<rightharpoonup> ('a vbpl_absval) bpl_val"
+type_synonym 'a bpl_mask_ty = "ref \<Rightarrow> 'a vb_field \<Rightarrow> real"
+
+
+definition heap_rel :: "ViperLang.program \<Rightarrow> 'a total_heap \<Rightarrow> 'a bpl_heap_ty \<Rightarrow> bool"
+  where "heap_rel Pr h hb \<equiv> 
+    \<forall> l :: heap_loc. if_Some 
+                       (\<lambda>field_vty. option_fold (\<lambda>res. val_rel_vpr_bpl (h l) res) False (hb (Address (fst l)) (NormalField (snd l) field_vty)))
+                       (declared_fields Pr (snd l))"
+
+definition mask_rel :: "ViperLang.program \<Rightarrow> mask \<Rightarrow> 'a bpl_mask_ty \<Rightarrow> bool"
+  where "mask_rel Pr m mb \<equiv> 
+    \<forall> l :: heap_loc. if_Some 
+                       (\<lambda>field_vty. real_of_rat (Rep_prat (m l)) = (mb (Address (fst l)) (NormalField (snd l) field_vty)))
+                       (declared_fields Pr (snd l))"
+
+(* TODO *)
+definition predicate_heap_rel :: "ViperLang.program \<Rightarrow> ('a \<Rightarrow> abs_type) \<Rightarrow> 'a predicate_heap \<Rightarrow> 'a bpl_heap_ty \<Rightarrow> bool"
+  where "predicate_heap_rel Pr A h hb \<equiv> 
+    \<forall> pred_id :: predicate_ident. \<forall> tys :: vtyp list. map_option (predicate_decl.args) (ViperLang.predicates Pr pred_id) = Some tys \<longrightarrow>
+        (\<forall>vs. map (get_type A) vs = tys \<longrightarrow> True) "
+
+(* TODO: lift to predicates *)
+definition state_rel_vpr_bpl :: "ViperLang.program \<Rightarrow> tr_vpr_bpl \<Rightarrow> 'a full_total_state \<Rightarrow> ('a vbpl_absval) nstate \<Rightarrow> bool"
+  where "state_rel_vpr_bpl Pr T \<omega> ns \<equiv>
+           (\<forall> var_vpr var_bpl. var_translation T var_vpr = Some var_bpl \<longrightarrow> 
+              (\<exists>val_vpr val_bpl. ((get_store_total \<omega>) var_vpr) = Some val_vpr \<and>
+                                ((local_state ns) var_vpr) = Some val_bpl \<and>
+                                val_rel_vpr_bpl val_vpr val_bpl)) \<and>
+           (\<exists>hb. (global_state ns) (heap_var T) = Some (AbsV (AHeap hb)) \<and> heap_rel Pr (get_hh_total_full \<omega>) hb) \<and>
+           (\<exists>mb. (global_state ns) (mask_var T) = Some (AbsV (AMask mb)) \<and> mask_rel Pr (get_mh_total_full \<omega>) mb)"
+
+definition exp_rel_vpr_bpl :: 
+   "ViperLang.program \<Rightarrow> 'a interp \<Rightarrow> 'a ty_repr_bpl \<Rightarrow> tr_vpr_bpl \<Rightarrow> var_context \<Rightarrow> ('a vbpl_absval) fun_interp \<Rightarrow> viper_expr \<Rightarrow> boogie_expr \<Rightarrow> 'a full_total_state \<Rightarrow> ('a vbpl_absval) nstate \<Rightarrow> bool"
+  where "exp_rel_vpr_bpl Pr \<Delta> T Tr \<Lambda> \<Gamma> e_vpr e_bpl \<omega> ns \<equiv> 
+             \<exists>v1 v2. (Pr, \<Delta>, None \<turnstile> \<langle>e_vpr; \<omega>\<rangle> [\<Down>]\<^sub>t Val v1) \<and> ((vbpl_absval_ty T),\<Lambda>,\<Gamma>,[] \<turnstile> \<langle>e_bpl, ns\<rangle> \<Down> v2) \<and> (val_rel_vpr_bpl v1 v2)"
+
+
+inductive exp_rel :: "viper_expr \<Rightarrow> boogie_expr \<Rightarrow> bool"
+  where
+      "exp_rel (ViperLang.Var x) (Lang.Var y)"
+    | "exp_rel (ViperLang.ELit lit) (Lang.Lit litb)"
+    | " \<lbrakk> unop_rel uop = uopb; exp_rel e eb \<rbrakk> \<Longrightarrow>
+           exp_rel (ViperLang.Unop uop e) (Lang.UnOp uopb eb)"
+    | " \<lbrakk> binop_rel bop = bopb; exp_rel e1 e1b; exp_rel e2 e2b \<rbrakk> \<Longrightarrow>
+           exp_rel (ViperLang.Binop e1 bop e2) (Lang.BinOp e1b bopb e2b)"
+  
+
+end
